log_map.fst
@@ -7,309 +7,267 @@ open Library
 
 module A = Alpha_map
 
-module G = Log
+module L = Log
 
-val pre_cond_merge_a1 : l:A.s G.s -> a:A.s G.s -> b:A.s G.s 
+val pre_cond_merge_a : l:A.s L.s -> a:A.s L.s -> b:A.s L.s 
                       -> Pure bool
                         (requires true)
                         (ensures (fun b1 -> (b1 = true <==> (forall e. A.mem_key_s e l ==> A.mem_key_s e a /\ A.mem_key_s e b) /\
-                        (forall ch. A.mem_key_s ch a \/ A.mem_key_s ch b ==> 
-                        (forall e. mem e (A.get_val_s #G.s #G.op #G.rval ch l) ==> mem e (A.get_val_s #G.s #G.op #G.rval ch a) /\ mem e (A.get_val_s #G.s #G.op #G.rval ch b)) /\
-                        (forall e e1. mem e (A.get_val_s #G.s #G.op #G.rval ch l) /\ mem e1 (G.diff_s (A.get_val_s #G.s #G.op #G.rval ch a) (A.get_val_s #G.s #G.op #G.rval ch l)) ==> G.fst e1 > G.fst e) /\
-                        (forall e e1. mem e (A.get_val_s #G.s #G.op #G.rval ch l) /\ mem e1 (G.diff_s (A.get_val_s #G.s #G.op #G.rval ch b) (A.get_val_s #G.s #G.op #G.rval ch l)) ==> G.fst e1 > G.fst e)))))
+                          (forall ch. A.mem_key_s ch a \/ A.mem_key_s ch b ==> 
+                            (L.pre_cond_merge (A.get_val_s #L.s #L.op #L.rval ch l) 
+                            (A.get_val_s #L.s #L.op #L.rval ch a) (A.get_val_s #L.s #L.op #L.rval ch b))))))
 
 #set-options "--z3rlimit 1000"
-let pre_cond_merge_a1 l a b = 
-  forallb (fun e -> A.mem_key_s (A.get_key_s #G.s e) a && A.mem_key_s (A.get_key_s #G.s e) b) l &&
-  forallb (fun ch -> (forallb (fun e -> mem e (A.get_val_s #G.s #G.op #G.rval ch a) && mem e (A.get_val_s #G.s #G.op #G.rval ch b)) (A.get_val_s #G.s #G.op #G.rval ch l)) &&
-  (forallb (fun e -> (forallb (fun e1 -> G.fst e1 > G.fst e) (G.diff_s (A.get_val_s #G.s #G.op #G.rval ch a) (A.get_val_s #G.s #G.op #G.rval ch l)))) (A.get_val_s #G.s #G.op #G.rval ch l)) &&
-  (forallb (fun e -> (forallb (fun e1 -> G.fst e1 > G.fst e) (G.diff_s (A.get_val_s #G.s #G.op #G.rval ch b) (A.get_val_s #G.s #G.op #G.rval ch l)))) (A.get_val_s #G.s #G.op #G.rval ch l))) (A.get_key_lst l a b)
+let pre_cond_merge_a l a b = 
+  forallb (fun e -> A.mem_key_s (A.get_key_s #L.s e) a && A.mem_key_s (A.get_key_s #L.s e) b) l &&
+  forallb (fun ch -> L.pre_cond_merge (A.get_val_s #L.s #L.op #L.rval ch l) (A.get_val_s #L.s #L.op #L.rval ch a)  (A.get_val_s #L.s #L.op #L.rval ch b)) (A.get_key_lst l a b)
 
-val pre_cond_merge_a2 : l:A.s G.s -> a:A.s G.s -> b:A.s G.s 
-                      -> Pure bool
-                        (requires true)
-                        (ensures (fun b1 -> (b1 = true <==> (forall ch. A.mem_key_s ch a \/ A.mem_key_s ch b ==> 
-                          (G.pre_cond_merge (A.get_val_s #G.s #G.op #G.rval ch l) 
-                          (A.get_val_s #G.s #G.op #G.rval ch a) (A.get_val_s #G.s #G.op #G.rval ch b)) /\
-                          (forall e. mem e (A.get_val_s #G.s #G.op #G.rval ch l) ==> mem e (A.get_val_s #G.s #G.op #G.rval ch a) /\ mem e (A.get_val_s #G.s #G.op #G.rval ch b)) /\
-            (forall e. mem e (G.diff_s (A.get_val_s #G.s #G.op #G.rval ch a) (A.get_val_s #G.s #G.op #G.rval ch l)) ==>
-                           not (G.mem_id_s (G.fst e) (G.diff_s (A.get_val_s #G.s #G.op #G.rval ch b) (A.get_val_s #G.s #G.op #G.rval ch l)))) /\
-            (forall e. mem e (G.diff_s (A.get_val_s #G.s #G.op #G.rval ch b) (A.get_val_s #G.s #G.op #G.rval ch l)) ==>
-                           not (G.mem_id_s (G.fst e) (G.diff_s (A.get_val_s #G.s #G.op #G.rval ch a) (A.get_val_s#G.s #G.op #G.rval ch l))))))))
-
-#set-options "--z3rlimit 1000"
-let pre_cond_merge_a2 l a b =
-  forallb (fun ch -> G.pre_cond_merge (A.get_val_s #G.s #G.op #G.rval ch l) (A.get_val_s #G.s #G.op #G.rval ch a) (A.get_val_s #G.s #G.op #G.rval ch b) &&
-  (forallb (fun e -> mem e (A.get_val_s #G.s #G.op #G.rval ch a) && mem e (A.get_val_s #G.s #G.op #G.rval ch b)) (A.get_val_s #G.s #G.op #G.rval ch l)) &&
-  (forallb (fun e -> not (G.mem_id_s (G.fst e) (G.diff_s (A.get_val_s #G.s #G.op #G.rval ch b) (A.get_val_s #G.s #G.op #G.rval ch l)))) (G.diff_s (A.get_val_s #G.s #G.op #G.rval ch a) (A.get_val_s #G.s #G.op #G.rval ch l))) &&
-  (forallb (fun e -> not (G.mem_id_s (G.fst e) (G.diff_s (A.get_val_s #G.s #G.op #G.rval ch a) (A.get_val_s#G.s #G.op #G.rval ch l)))) (G.diff_s (A.get_val_s #G.s #G.op #G.rval ch b) (A.get_val_s #G.s #G.op #G.rval ch l)))) (A.get_key_lst l a b)
-
-val pre_cond_merge_a : l:A.s G.s -> a:A.s G.s -> b:A.s G.s 
-                      -> Pure bool
-                        (requires true)
-                        (ensures (fun b1 -> (b1 = true <==> (forall e. A.mem_key_s e l ==> A.mem_key_s e a /\ A.mem_key_s e b) /\
-                        (forall ch. A.mem_key_s ch a \/ A.mem_key_s ch b ==> 
-                          (G.pre_cond_merge (A.get_val_s #G.s #G.op #G.rval ch l) 
-                          (A.get_val_s #G.s #G.op #G.rval ch a) (A.get_val_s #G.s #G.op #G.rval ch b)) /\
-                          (forall e. mem e (A.get_val_s #G.s #G.op #G.rval ch l) ==> mem e (A.get_val_s #G.s #G.op #G.rval ch a) /\ mem e (A.get_val_s #G.s #G.op #G.rval ch b)) /\
-            (forall e. mem e (G.diff_s (A.get_val_s #G.s #G.op #G.rval ch a) (A.get_val_s #G.s #G.op #G.rval ch l)) ==>
-                           not (G.mem_id_s (G.fst e) (G.diff_s (A.get_val_s #G.s #G.op #G.rval ch b) (A.get_val_s #G.s #G.op #G.rval ch l)))) /\
-            (forall e. mem e (G.diff_s (A.get_val_s #G.s #G.op #G.rval ch b) (A.get_val_s #G.s #G.op #G.rval ch l)) ==>
-                           not (G.mem_id_s (G.fst e) (G.diff_s (A.get_val_s #G.s #G.op #G.rval ch a) (A.get_val_s#G.s #G.op #G.rval ch l)))) /\
-            (forall e e1. mem e (A.get_val_s #G.s #G.op #G.rval ch l) /\ mem e1 (G.diff_s (A.get_val_s #G.s #G.op #G.rval ch a) (A.get_val_s #G.s #G.op #G.rval ch l)) ==> G.fst e1 > G.fst e) /\
-            (forall e e1. mem e (A.get_val_s #G.s #G.op #G.rval ch l) /\ mem e1 (G.diff_s (A.get_val_s #G.s #G.op #G.rval ch b) (A.get_val_s #G.s #G.op #G.rval ch l)) ==> G.fst e1 > G.fst e)))))
-
-let pre_cond_merge_a l a b =
-  pre_cond_merge_a1 l a b &&
-  pre_cond_merge_a2 l a b
-
-val merge_a : l:A.s G.s
-             -> a:A.s G.s
-             -> b:A.s G.s
-             -> Pure (A.s G.s)
+val merge_a : l:A.s L.s
+             -> a:A.s L.s
+             -> b:A.s L.s
+             -> Pure (A.s L.s)
                (requires pre_cond_merge_a l a b)
                (ensures (fun r -> (forall ch. A.mem_key_s ch r <==> A.mem_key_s ch a \/ A.mem_key_s ch b) /\ A.unique_key r /\
-                               (forall ch. A.mem_key_s ch a \/ A.mem_key_s ch b ==> (A.get_val_s #G.s #G.op #G.rval ch r) =
-                               (G.merge (A.get_val_s #G.s #G.op #G.rval ch l) (A.get_val_s #G.s #G.op #G.rval ch a) (A.get_val_s #G.s #G.op #G.rval ch b)))))
+                               (forall ch. A.mem_key_s ch a \/ A.mem_key_s ch b ==> (A.get_val_s #L.s #L.op #L.rval ch r) =
+                               (L.merge (A.get_val_s #L.s #L.op #L.rval ch l) (A.get_val_s #L.s #L.op #L.rval ch a) (A.get_val_s #L.s #L.op #L.rval ch b)))))
 
-let merge_a l a b = A.merge_a #G.s #G.op #G.rval l a b
+let merge_a l a b = A.merge_a #L.s #L.op #L.rval l a b
 
-val lemma2 : s1:A.s G.s
+val lemma2 : s1:A.s L.s
            -> Lemma (requires true)
-                   (ensures (forall e. mem e s1 ==> (A.get_val_s #G.s #G.op #G.rval (A.get_key_s e) s1 = A.get_val_s1 #G.s e)))
+                   (ensures (forall e. mem e s1 ==> (A.get_val_s #L.s #L.op #L.rval (A.get_key_s e) s1 = A.get_val_s1 #L.s e)))
 let rec lemma2 s1 =
   match s1 with
   |[] -> ()
   |x::xs -> lemma2 xs
 
-val lemma4 : tr:ae (A.op G.op) -> s1:A.s G.s
-           -> Lemma (requires A.sim_a #G.s #G.op #G.rval tr s1)
-                   (ensures (forall i. (G.sim (A.project i tr) (A.get_val_s #G.s #G.op #G.rval i s1))))
+val lemma4 : tr:ae (A.op L.op) -> s1:A.s L.s
+           -> Lemma (requires A.sim_a #L.s #L.op #L.rval tr s1)
+                   (ensures (forall i. (L.sim (A.project i tr) (A.get_val_s #L.s #L.op #L.rval i s1))))
 let lemma4 tr s1 = ()
 
-val lemma1 : tr:ae (A.op G.op)
-         -> st:A.s G.s
-         -> op1:(nat * (A.op G.op))
-         -> Lemma (requires (A.sim_a #G.s #G.op #G.rval tr st) /\ (not (mem_id (get_id op1) tr.l)) /\
+val lemma1 : tr:ae (A.op L.op)
+         -> st:A.s L.s
+         -> op1:(nat * (A.op L.op))
+         -> Lemma (requires (A.sim_a #L.s #L.op #L.rval tr st) /\ (not (mem_id (get_id op1) tr.l)) /\
                            (forall e. mem e tr.l ==> get_id e < get_id op1) /\ get_id op1 > 0 /\
-                          G.pre_cond_do (A.get_val_s #G.s #G.op #G.rval (A.get_key op1) st) (A.project_op op1))
-                 (ensures (forall i. A.mem_key_s i (get_st (A.do_a #G.s #G.op #G.rval st op1)) /\ i <> A.get_key op1 ==>
+                          L.pre_cond_do (A.get_val_s #L.s #L.op #L.rval (A.get_key op1) st) (A.project_op op1))
+                 (ensures (forall i. A.mem_key_s i (get_st (A.do_a #L.s #L.op #L.rval st op1)) /\ i <> A.get_key op1 ==>
                  ((forall e. mem e (A.project i (abs_do tr op1)).l <==> mem e (A.project i tr).l) /\
              (forall e e1. mem e (A.project i (abs_do tr op1)).l /\ mem e1 (A.project i (abs_do tr op1)).l /\ get_id e <> get_id e1 /\
                       (A.project i (abs_do tr op1)).vis e e1 <==> 
                  mem e (A.project i tr).l /\ mem e1 (A.project i tr).l /\ get_id e <> get_id e1 /\ (A.project i tr).vis e e1) /\
-             (A.get_val_s #G.s #G.op #G.rval i (get_st (A.do_a #G.s #G.op #G.rval st op1)) = (A.get_val_s #G.s #G.op #G.rval i st))) ==>
-                          (G.sim (A.project i (abs_do tr op1)) (A.get_val_s #G.s #G.op #G.rval i (get_st (A.do_a #G.s #G.op #G.rval st op1))))))
+             (A.get_val_s #L.s #L.op #L.rval i (get_st (A.do_a #L.s #L.op #L.rval st op1)) = (A.get_val_s #L.s #L.op #L.rval i st))) ==>
+                          (L.sim (A.project i (abs_do tr op1)) (A.get_val_s #L.s #L.op #L.rval i (get_st (A.do_a #L.s #L.op #L.rval st op1))))))
 
 #set-options "--z3rlimit 1000"
 let lemma1 tr st op = ()
 
-val lemma7 : tr:ae G.op -> s1:G.s -> tr1:ae G.op
-           -> Lemma (requires G.sim tr s1 /\ (forall e. mem e tr1.l <==> mem e tr.l) /\
+val lemma7 : tr:ae L.op -> s1:L.s -> tr1:ae L.op
+           -> Lemma (requires L.sim tr s1 /\ (forall e. mem e tr1.l <==> mem e tr.l) /\
                              (forall e e1. mem e tr1.l /\ mem e1 tr1.l /\ get_id e <> get_id e1 /\ tr1.vis e e1 <==>
                                       mem e tr.l /\ mem e1 tr.l /\ get_id e <> get_id e1 /\ tr.vis e e1))
-                   (ensures (G.sim tr1 s1))
+                   (ensures (L.sim tr1 s1))
 #set-options "--z3rlimit 1000"
 let lemma7 tr s1 tr1 = ()
 
-instance _ : A.alpha_map G.s G.op G.rval G.log = {
+instance _ : A.alpha_map L.s L.op L.rval L.log = {
   A.lemma1 = lemma1;
   A.lemma4 = lemma4;
   A.lemma2 = lemma2;
   A.lemma7 = lemma7
 }
 
-val pre_cond_prop_merge_a : ltr:ae (A.op G.op) 
-                     -> l:A.s G.s 
-                     -> atr:ae (A.op G.op)
-                     -> a:A.s G.s 
-                     -> btr:ae (A.op G.op)
-                     -> b:A.s G.s
+val pre_cond_prop_merge_a : ltr:ae (A.op L.op) 
+                     -> l:A.s L.s 
+                     -> atr:ae (A.op L.op)
+                     -> a:A.s L.s 
+                     -> btr:ae (A.op L.op)
+                     -> b:A.s L.s
                      -> Tot (b1:bool {b1=true <==> (forall ch. A.mem_key_s ch a \/ A.mem_key_s ch b ==>
-                          (G.pre_cond_prop_merge (A.project ch ltr) (A.get_val_s #G.s #G.op #G.rval ch l)
-                                            (A.project ch atr) (A.get_val_s #G.s #G.op #G.rval ch a)
-                                            (A.project ch btr) (A.get_val_s #G.s #G.op #G.rval ch b)) /\
+                          (L.pre_cond_prop_merge (A.project ch ltr) (A.get_val_s #L.s #L.op #L.rval ch l)
+                                                 (A.project ch atr) (A.get_val_s #L.s #L.op #L.rval ch a)
+                                                 (A.project ch btr) (A.get_val_s #L.s #L.op #L.rval ch b)) /\
                               (forall e. mem e (A.project ch ltr).l ==> not (mem_id (get_id e) (A.project ch atr).l)) /\
                               (forall e. mem e (A.project ch atr).l ==> not (mem_id (get_id e) (A.project ch btr).l)) /\
                               (forall e. mem e (A.project ch ltr).l ==> not (mem_id (get_id e) (A.project ch btr).l)) /\
-                                (G.sim (A.project ch ltr) (A.get_val_s #G.s #G.op #G.rval ch l) /\ 
-                      G.sim (union (A.project ch ltr) (A.project ch atr)) (A.get_val_s #G.s #G.op #G.rval ch a) /\
-                     G.sim (union (A.project ch ltr) (A.project ch btr)) (A.get_val_s #G.s #G.op #G.rval ch b)))})
+                     (L.sim (A.project ch ltr) (A.get_val_s #L.s #L.op #L.rval ch l) /\ 
+                      L.sim (union (A.project ch ltr) (A.project ch atr)) (A.get_val_s #L.s #L.op #L.rval ch a) /\
+                      L.sim (union (A.project ch ltr) (A.project ch btr)) (A.get_val_s #L.s #L.op #L.rval ch b)))})
 
 let pre_cond_prop_merge_a ltr l atr a btr b =
-  forallb (fun ch -> (G.pre_cond_prop_merge (A.project ch ltr) (A.get_val_s #G.s #G.op #G.rval ch l)
-                                    (A.project ch atr) (A.get_val_s #G.s #G.op #G.rval ch a)
-                                    (A.project ch btr) (A.get_val_s #G.s #G.op #G.rval ch b)) &&
-  (forallb (fun e -> not (mem_id (get_id e) (A.project ch atr).l)) (A.project ch ltr).l) &&
-  (forallb (fun e -> not (mem_id (get_id e) (A.project ch btr).l)) (A.project ch atr).l) &&
-  (forallb (fun e -> not (mem_id (get_id e) (A.project ch btr).l)) (A.project ch ltr).l) &&
-  (G.sim (A.project ch ltr) (A.get_val_s #G.s #G.op #G.rval ch l)) &&
-  (G.sim (union (A.project ch ltr) (A.project ch atr)) (A.get_val_s #G.s #G.op #G.rval ch a)) &&
-  (G.sim (union (A.project ch ltr) (A.project ch btr)) (A.get_val_s #G.s #G.op #G.rval ch b))) (A.get_key_lst l a b)
+  forallb (fun ch -> (L.pre_cond_prop_merge (A.project ch ltr) (A.get_val_s #L.s #L.op #L.rval ch l)
+                                    (A.project ch atr) (A.get_val_s #L.s #L.op #L.rval ch a)
+                                    (A.project ch btr) (A.get_val_s #L.s #L.op #L.rval ch b)) &&
+  forallb (fun e -> not (mem_id (get_id e) (A.project ch atr).l)) (A.project ch ltr).l &&
+  forallb (fun e -> not (mem_id (get_id e) (A.project ch btr).l)) (A.project ch atr).l &&
+  forallb (fun e -> not (mem_id (get_id e) (A.project ch btr).l)) (A.project ch ltr).l &&
+  L.sim (A.project ch ltr) (A.get_val_s #L.s #L.op #L.rval ch l) &&
+  L.sim (union (A.project ch ltr) (A.project ch atr)) (A.get_val_s #L.s #L.op #L.rval ch a) &&
+  L.sim (union (A.project ch ltr) (A.project ch btr)) (A.get_val_s #L.s #L.op #L.rval ch b)) (A.get_key_lst l a b)
 
-val pre_cond_do_a : s1:(A.s G.s) -> op1:(nat * (A.op G.op))
+val pre_cond_do_a : s1:(A.s L.s) -> op1:(nat * (A.op L.op))
                   -> Tot (b:bool {b = true <==> 
-                        G.pre_cond_do (A.get_val_s #G.s #G.op #G.rval (A.get_key op1) s1) (A.project_op op1)})
+                        L.pre_cond_do (A.get_val_s #L.s #L.op #L.rval (A.get_key op1) s1) (A.project_op op1)})
 let pre_cond_do_a s1 op = 
-  G.pre_cond_do (A.get_val_s #G.s #G.op #G.rval (A.get_key op) s1) (A.project_op op)
+  L.pre_cond_do (A.get_val_s #L.s #L.op #L.rval (A.get_key op) s1) (A.project_op op)
 
-val pre_cond_prop_do_a : tr:ae (A.op G.op)
-                       -> st:(A.s G.s)
-                       -> op1:(nat * (A.op G.op)) 
+val pre_cond_prop_do_a : tr:ae (A.op L.op)
+                       -> st:(A.s L.s)
+                       -> op1:(nat * (A.op L.op)) 
                        -> Pure bool
                          (requires (not (mem_id (get_id op1) tr.l) /\
                                    (forall e. mem e tr.l ==> get_id e < get_id op1) /\ get_id op1 > 0))
-                         (ensures (fun b -> (b=true <==> (G.pre_cond_prop_do (A.project (A.get_key op1) (abs_do tr op1))
-                                  (A.get_val_s #G.s #G.op #G.rval (A.get_key op1) st) (A.project_op op1)) /\
-                              G.pre_cond_do (A.get_val_s #G.s #G.op #G.rval (A.get_key op1) st) (A.project_op op1) /\
-                           (G.sim (A.project (A.get_key op1) (abs_do tr op1)) (A.get_val_s #G.s #G.op #G.rval (A.get_key op1) (get_st (A.do_a #G.s #G.op #G.rval st op1)))))))
+                         (ensures (fun b -> (b=true <==> (L.pre_cond_prop_do (A.project (A.get_key op1) tr)
+                                  (A.get_val_s #L.s #L.op #L.rval (A.get_key op1) st) (A.project_op op1)) /\
+                              L.pre_cond_do (A.get_val_s #L.s #L.op #L.rval (A.get_key op1) st) (A.project_op op1) /\
+                           (L.sim (A.project (A.get_key op1) (abs_do tr op1)) (A.get_val_s #L.s #L.op #L.rval (A.get_key op1) (get_st (A.do_a #L.s #L.op #L.rval st op1)))))))
 
 let pre_cond_prop_do_a tr st op1 =
-    G.pre_cond_prop_do (A.project (A.get_key op1) (abs_do tr op1))
-                         (A.get_val_s #G.s #G.op #G.rval (A.get_key op1) st) (A.project_op op1) &&
-    G.pre_cond_do (A.get_val_s #G.s #G.op #G.rval (A.get_key op1) st) (A.project_op op1) &&
-    G.sim (A.project (A.get_key op1) (abs_do tr op1)) (A.get_val_s #G.s #G.op #G.rval (A.get_key op1) 
-                     (get_st (A.do_a #G.s #G.op #G.rval st op1)))
+    L.pre_cond_prop_do (A.project (A.get_key op1) tr)
+                         (A.get_val_s #L.s #L.op #L.rval (A.get_key op1) st) (A.project_op op1) &&
+    L.pre_cond_do (A.get_val_s #L.s #L.op #L.rval (A.get_key op1) st) (A.project_op op1) &&
+    L.sim (A.project (A.get_key op1) (abs_do tr op1)) (A.get_val_s #L.s #L.op #L.rval (A.get_key op1) 
+                     (get_st (A.do_a #L.s #L.op #L.rval st op1)))
 
-val prop_do_a : tr:ae (A.op G.op)
-              -> st:A.s G.s
-              -> op1:(nat * (A.op G.op)) 
-              -> Lemma (requires (A.sim_a #G.s #G.op #G.rval tr st) /\ (not (mem_id (get_id op1) tr.l)) /\
+val prop_do_a : tr:ae (A.op L.op)
+              -> st:A.s L.s
+              -> op1:(nat * (A.op L.op)) 
+              -> Lemma (requires (A.sim_a #L.s #L.op #L.rval tr st) /\ (not (mem_id (get_id op1) tr.l)) /\
                                 (forall e. mem e tr.l ==> get_id e < get_id op1) /\ get_id op1 > 0 /\
                                 pre_cond_do_a st op1 /\ pre_cond_prop_do_a tr st op1)
-                      (ensures (A.sim_a #G.s #G.op #G.rval (abs_do tr op1) (get_st (A.do_a #G.s #G.op #G.rval st op1))))
+                      (ensures (A.sim_a #L.s #L.op #L.rval (abs_do tr op1) (get_st (A.do_a #L.s #L.op #L.rval st op1))))
 
 #set-options "--z3rlimit 1000"
 let prop_do_a tr st op = 
-  A.prop_do_a #G.s #G.op #G.rval #G.log tr st op
+  A.prop_do_a #L.s #L.op #L.rval #L.log tr st op
 
-val convergence2 : tr:ae (A.op G.op)
-                 -> a:(A.s G.s)
-                 -> b:(A.s G.s)
-                 -> Lemma (requires (A.sim_a #G.s #G.op #G.rval tr a /\ A.sim_a #G.s #G.op #G.rval tr b))
+val convergence2 : tr:ae (A.op L.op)
+                 -> a:(A.s L.s)
+                 -> b:(A.s L.s)
+                 -> Lemma (requires (A.sim_a #L.s #L.op #L.rval tr a /\ A.sim_a #L.s #L.op #L.rval tr b))
                          (ensures (forall ch. A.mem_key_s ch a /\ A.mem_key_s ch b ==> 
-         (forall e e1. mem e (A.get_val_s #G.s #G.op #G.rval ch a) /\ mem e1 (A.get_val_s #G.s #G.op #G.rval ch a) /\ 
-                    G.fst e <> G.fst e1 /\ G.fst e > G.fst e1 /\ G.ord e e1 (A.get_val_s #G.s #G.op #G.rval ch a)  <==> 
-    mem e (A.get_val_s #G.s #G.op #G.rval ch b) /\ mem e1 (A.get_val_s #G.s #G.op #G.rval ch b) /\ G.fst e <> G.fst e1 /\
-                    G.fst e > G.fst e1 /\ G.ord e e1 (A.get_val_s #G.s #G.op #G.rval ch b))) /\
+         (forall e e1. mem e (A.get_val_s #L.s #L.op #L.rval ch a) /\ mem e1 (A.get_val_s #L.s #L.op #L.rval ch a) /\ 
+                    L.fst e <> L.fst e1 /\ L.fst e > L.fst e1 /\ L.ord e e1 (A.get_val_s #L.s #L.op #L.rval ch a)  <==> 
+    mem e (A.get_val_s #L.s #L.op #L.rval ch b) /\ mem e1 (A.get_val_s #L.s #L.op #L.rval ch b) /\ L.fst e <> L.fst e1 /\
+                    L.fst e > L.fst e1 /\ L.ord e e1 (A.get_val_s #L.s #L.op #L.rval ch b))) /\
           (forall ch. A.mem_key_s ch a /\ A.mem_key_s ch b ==>
-    (forall e. G.mem_id_s e (A.get_val_s #G.s #G.op #G.rval ch a) <==> G.mem_id_s e (A.get_val_s #G.s #G.op #G.rval ch b))))
+    (forall e. L.mem_id_s e (A.get_val_s #L.s #L.op #L.rval ch a) <==> L.mem_id_s e (A.get_val_s #L.s #L.op #L.rval ch b))))
 
 #set-options "--z3rlimit 1000"
 let convergence2 tr a b = 
-  A.convergence_a1 #G.s #G.op #G.rval tr a b
+  A.convergence_a1 #L.s #L.op #L.rval tr a b
 
-val lem_length : a:(A.s G.s)
-               -> b:(A.s G.s)
+val lem_length : a:(A.s L.s)
+               -> b:(A.s L.s)
                -> lst:list nat
                -> Lemma (requires (forall ch. mem ch lst ==> A.mem_key_s ch a /\ A.mem_key_s ch b) /\
                                           (forall e. A.mem_key_s e a <==> A.mem_key_s e b) /\
                                     A.unique_keys lst /\ (forall ch. mem ch lst ==> 
-                 (forall e. G.mem_id_s e (A.get_val_s #G.s #G.op #G.rval ch a) <==> G.mem_id_s e (A.get_val_s #G.s #G.op #G.rval ch b))))
-                 (ensures (forall ch. mem ch lst ==> (List.Tot.length (A.get_val_s #G.s #G.op #G.rval ch a) = List.Tot.length (A.get_val_s #G.s #G.op #G.rval ch b))))
+                 (forall e. L.mem_id_s e (A.get_val_s #L.s #L.op #L.rval ch a) <==> L.mem_id_s e (A.get_val_s #L.s #L.op #L.rval ch b))))
+                 (ensures (forall ch. mem ch lst ==> (List.Tot.length (A.get_val_s #L.s #L.op #L.rval ch a) = List.Tot.length (A.get_val_s #L.s #L.op #L.rval ch b))))
                           (decreases lst)
 
 let rec lem_length a b lst =
   match lst with
   |[] -> ()
-  |ch::chs -> G.lem_length (A.get_val_s #G.s #G.op #G.rval ch a) (A.get_val_s #G.s #G.op #G.rval ch b); 
+  |ch::chs -> L.lem_length (A.get_val_s #L.s #L.op #L.rval ch a) (A.get_val_s #L.s #L.op #L.rval ch b); 
             lem_length a b chs
 
-val convergence3 : a:(A.s G.s)
-                 -> b:(A.s G.s)
+val convergence3 : a:(A.s L.s)
+                 -> b:(A.s L.s)
                  -> lst:list nat
                  -> Lemma (requires (forall ch. mem ch lst ==> A.mem_key_s ch a /\ A.mem_key_s ch b) /\
                                    (forall e. A.mem_key_s e a <==> A.mem_key_s e b) /\
                                     A.unique_keys lst /\ (forall ch. mem ch lst ==> 
-    (forall e. G.mem_id_s e (A.get_val_s #G.s #G.op #G.rval ch a) <==> G.mem_id_s e (A.get_val_s #G.s #G.op #G.rval ch b))) /\
-    (forall ch. mem ch lst ==> (forall e. mem e (A.get_val_s #G.s #G.op #G.rval ch a) <==> mem e (A.get_val_s #G.s #G.op #G.rval ch b))) /\
-                   (forall ch. mem ch lst ==> (List.Tot.length (A.get_val_s #G.s #G.op #G.rval ch a) = List.Tot.length (A.get_val_s #G.s #G.op #G.rval ch b))) /\
+    (forall e. L.mem_id_s e (A.get_val_s #L.s #L.op #L.rval ch a) <==> L.mem_id_s e (A.get_val_s #L.s #L.op #L.rval ch b))) /\
+    (forall ch. mem ch lst ==> (forall e. mem e (A.get_val_s #L.s #L.op #L.rval ch a) <==> mem e (A.get_val_s #L.s #L.op #L.rval ch b))) /\
+                   (forall ch. mem ch lst ==> (List.Tot.length (A.get_val_s #L.s #L.op #L.rval ch a) = List.Tot.length (A.get_val_s #L.s #L.op #L.rval ch b))) /\
                     (forall ch. mem ch lst ==> 
-           (forall e e1. mem e (A.get_val_s #G.s #G.op #G.rval ch a) /\ mem e1 (A.get_val_s #G.s #G.op #G.rval ch a) /\ 
-                   G.fst e <> G.fst e1 /\ G.fst e > G.fst e1 /\ G.ord e e1 (A.get_val_s #G.s #G.op #G.rval ch a)  <==> 
-                   mem e (A.get_val_s #G.s #G.op #G.rval ch b) /\ mem e1 (A.get_val_s #G.s #G.op #G.rval ch b) /\ 
-                   G.fst e <> G.fst e1 /\ G.fst e > G.fst e1 /\ G.ord e e1 (A.get_val_s #G.s #G.op #G.rval ch b))))
-                          (ensures (forall ch. mem ch lst ==> (A.get_val_s #G.s #G.op #G.rval ch a = 
-                                                         A.get_val_s #G.s #G.op #G.rval ch b)))
+           (forall e e1. mem e (A.get_val_s #L.s #L.op #L.rval ch a) /\ mem e1 (A.get_val_s #L.s #L.op #L.rval ch a) /\ 
+                   L.fst e <> L.fst e1 /\ L.fst e > L.fst e1 /\ L.ord e e1 (A.get_val_s #L.s #L.op #L.rval ch a)  <==> 
+                   mem e (A.get_val_s #L.s #L.op #L.rval ch b) /\ mem e1 (A.get_val_s #L.s #L.op #L.rval ch b) /\ 
+                   L.fst e <> L.fst e1 /\ L.fst e > L.fst e1 /\ L.ord e e1 (A.get_val_s #L.s #L.op #L.rval ch b))))
+                          (ensures (forall ch. mem ch lst ==> (A.get_val_s #L.s #L.op #L.rval ch a = 
+                                                         A.get_val_s #L.s #L.op #L.rval ch b)))
                          (decreases lst)
 #set-options "--z3rlimit 10000"
 let rec convergence3 a b lst =
   match lst with
   |[] -> ()
-  |ch::chs -> G.lem_same (A.get_val_s #G.s #G.op #G.rval ch a) (A.get_val_s #G.s #G.op #G.rval ch b);
+  |ch::chs -> L.lem_same (A.get_val_s #L.s #L.op #L.rval ch a) (A.get_val_s #L.s #L.op #L.rval ch b);
             convergence3 a b chs
 
-val convergence_a : tr:ae (A.op G.op)
-                  -> a:A.s G.s
-                  -> b:A.s G.s
-                  -> Lemma (requires (A.sim_a #G.s #G.op #G.rval tr a /\ A.sim_a #G.s #G.op #G.rval tr b))
+val convergence_a : tr:ae (A.op L.op)
+                  -> a:A.s L.s
+                  -> b:A.s L.s
+                  -> Lemma (requires (A.sim_a #L.s #L.op #L.rval tr a /\ A.sim_a #L.s #L.op #L.rval tr b))
                           (ensures (forall e. A.mem_key_s e a <==> A.mem_key_s e b) /\
                                    (forall ch. A.mem_key_s ch a /\ A.mem_key_s ch b ==> 
-                                   (A.get_val_s #G.s #G.op #G.rval ch a) = (A.get_val_s #G.s #G.op #G.rval ch b)))
+                                   (A.get_val_s #L.s #L.op #L.rval ch a) = (A.get_val_s #L.s #L.op #L.rval ch b)))
 
 #set-options "--z3rlimit 1000"
 let convergence_a tr a b = 
-  A.convergence_a1 #G.s #G.op #G.rval  tr a b;
+  A.convergence_a1 #L.s #L.op #L.rval  tr a b;
   convergence2 tr a b;
   lem_length a b (A.get_lst a);
   convergence3 a b (A.get_lst a)
 
-val prop_merge_a : ltr:ae (A.op G.op)
-            -> l:(A.s G.s)
-            -> atr:ae (A.op G.op)
-            -> a:(A.s G.s)
-            -> btr:ae (A.op G.op)
-            -> b:(A.s G.s)
+val prop_merge_a : ltr:ae (A.op L.op)
+            -> l:(A.s L.s)
+            -> atr:ae (A.op L.op)
+            -> a:(A.s L.s)
+            -> btr:ae (A.op L.op)
+            -> b:(A.s L.s)
             -> Lemma (requires (forall e. mem e ltr.l ==> not (mem_id (get_id e) atr.l)) /\
-                            (forall e. mem e atr.l ==> not (mem_id (get_id e) btr.l)) /\
-                            (forall e. mem e ltr.l ==> not (mem_id (get_id e) btr.l)) /\
-                            (A.sim_a #G.s #G.op #G.rval ltr l /\ A.sim_a #G.s #G.op #G.rval (union ltr atr) a /\ A.sim_a #G.s #G.op #G.rval (union ltr btr) b) /\
-                             pre_cond_merge_a l a b /\
+                              (forall e. mem e atr.l ==> not (mem_id (get_id e) btr.l)) /\
+                              (forall e. mem e ltr.l ==> not (mem_id (get_id e) btr.l)) /\
+                              (A.sim_a #L.s #L.op #L.rval ltr l /\ 
+                              A.sim_a #L.s #L.op #L.rval (union ltr atr) a /\
+                              A.sim_a #L.s #L.op #L.rval (union ltr btr) b) /\
+                              pre_cond_merge_a l a b /\
                              (forall ch. A.mem_key_s ch a \/ A.mem_key_s ch b ==> 
-                         (pre_cond_prop_merge #G.s #G.op #G.rval (A.project ch ltr) (A.get_val_s #G.s #G.op #G.rval ch l)
-                                             (A.project ch atr) (A.get_val_s #G.s #G.op #G.rval ch a)
-                                             (A.project ch btr) (A.get_val_s #G.s #G.op #G.rval ch b)) /\
-                            (forall e. mem e (A.project ch ltr).l ==> not (mem_id (get_id e) (A.project ch atr).l)) /\
-                            (forall e. mem e (A.project ch atr).l ==> not (mem_id (get_id e) (A.project ch btr).l)) /\
-                            (forall e. mem e (A.project ch ltr).l ==> not (mem_id (get_id e) (A.project ch btr).l)) /\
-                (sim #G.s #G.op #G.rval (A.project ch ltr) (A.get_val_s #G.s #G.op #G.rval ch l) /\ sim #G.s #G.op #G.rval (union (A.project ch ltr) (A.project ch atr)) (A.get_val_s #G.s #G.op #G.rval ch a) /\ sim #G.s #G.op #G.rval (union (A.project ch ltr) (A.project ch btr)) (A.get_val_s #G.s #G.op #G.rval ch b))))
-                (ensures (A.sim_a #G.s #G.op #G.rval (abs_merge ltr atr btr) (merge_a l a b)))
+                (pre_cond_prop_merge #L.s #L.op #L.rval (A.project ch ltr) (A.get_val_s #L.s #L.op #L.rval ch l)
+                                                        (A.project ch atr) (A.get_val_s #L.s #L.op #L.rval ch a)
+                                                        (A.project ch btr) (A.get_val_s #L.s #L.op #L.rval ch b)) /\
+                (sim #L.s #L.op #L.rval (A.project ch ltr) (A.get_val_s #L.s #L.op #L.rval ch l) /\ sim #L.s #L.op #L.rval (union (A.project ch ltr) (A.project ch atr)) (A.get_val_s #L.s #L.op #L.rval ch a) /\ sim #L.s #L.op #L.rval (union (A.project ch ltr) (A.project ch btr)) (A.get_val_s #L.s #L.op #L.rval ch b))))
+                (ensures (A.sim_a #L.s #L.op #L.rval (abs_merge ltr atr btr) (merge_a l a b)))
 
 #set-options "--z3rlimit 1000"
 let prop_merge_a ltr l atr a btr b = 
-  A.prop_merge_a #G.s #G.op #G.rval #G.log ltr l atr a btr b
+  A.prop_merge_a #L.s #L.op #L.rval #L.log ltr l atr a btr b
 
-val extract : r:G.rval {r <> G.Bot} -> G.s
-let extract (G.Val s) = s
+val extract : r:L.rval {r <> L.Bot} -> L.s
+let extract (L.Val s) = s
 
-val spec_a : o1:(nat * (A.op G.op))
-           -> tr:ae (A.op G.op)
-           -> Pure G.rval
+val spec_a : o1:(nat * (A.op L.op))
+           -> tr:ae (A.op L.op)
+           -> Pure L.rval
              (requires true)
-             (ensures (fun res -> A.opget o1 ==> (res = G.spec (A.project_op o1) (A.project (A.get_key o1) tr))))
-let spec_a o1 tr = G.spec (A.project_op o1) (A.project (A.get_key o1) tr)
+             (ensures (fun res -> A.opget o1 ==> (res = L.spec (A.project_op o1) (A.project (A.get_key o1) tr))))
+let spec_a o1 tr = L.spec (A.project_op o1) (A.project (A.get_key o1) tr)
 
-val prop_spec_a : tr:ae (A.op G.op)
-                  -> st1:(A.s G.s)
-                  -> op:(nat * (A.op G.op))
-                  -> Lemma (requires (A.sim_a #G.s #G.op #G.rval tr st1) /\ (not (mem_id (get_id op) tr.l)) /\
+val prop_spec_a : tr:ae (A.op L.op)
+                  -> st1:(A.s L.s)
+                  -> op:(nat * (A.op L.op))
+                  -> Lemma (requires (A.sim_a #L.s #L.op #L.rval tr st1) /\ (not (mem_id (get_id op) tr.l)) /\
                                     (forall e. mem e tr.l ==> get_id e < get_id op) /\ get_id op > 0 /\
                                     pre_cond_do_a st1 op)
-                    (ensures A.opget op ==> (get_rval (A.do_a #G.s #G.op #G.rval st1 op)) =
-                                                  ((A.spec_a #G.s #G.op #G.rval) op tr))
+                    (ensures A.opget op ==> (get_rval (A.do_a #L.s #L.op #L.rval st1 op)) =
+                                                  ((A.spec_a #L.s #L.op #L.rval) op tr))
 
 #set-options "--z3rlimit 1000"
 let prop_spec_a tr st op =
-  G.prop_spec (A.project (A.get_key op) tr) (A.get_val_s #G.s #G.op #G.rval (A.get_key op) st) (A.project_op op)
+  L.prop_spec (A.project (A.get_key op) tr) (A.get_val_s #L.s #L.op #L.rval (A.get_key op) st) (A.project_op op)
 
-val sim_a : tr:ae (A.op G.op)
-          -> s1:(A.s G.s)
+val sim_a : tr:ae (A.op L.op)
+          -> s1:(A.s L.s)
           -> Tot (b:bool {(b = true) <==> (forall e1. mem e1 s1 ==> (exists e. mem e tr.l /\ A.get_key_s e1 = A.get_key e /\ A.opset e)) /\
-                (forall k. A.mem_key_s k s1 ==> G.sim (A.project k tr) (A.get_val_s #G.s #G.op #G.rval k s1)) /\
+                (forall k. A.mem_key_s k s1 ==> L.sim (A.project k tr) (A.get_val_s #L.s #L.op #L.rval k s1)) /\
               (forall e. mem e tr.l /\ A.opset e ==> (exists e1. mem e1 s1 /\ A.get_key e = A.get_key_s e1))})
-let sim_a tr s1 = A.sim_a #G.s #G.op #G.rval tr s1
+let sim_a tr s1 = A.sim_a #L.s #L.op #L.rval tr s1
 
-instance log_map : mrdt (A.s G.s) (A.op G.op) (G.rval) = {
+instance log_map : mrdt (A.s L.s) (A.op L.op) (L.rval) = {
   Library.init = A.init_a;
   Library.spec = spec_a;
   Library.sim = sim_a;
